TensorLib/Bytes.lean
@@ -12,16 +12,17 @@ namespace TensorLib
 -- as a Nat at runtime. We'll have tests for these in our ByteArray extension module where we
 -- have conversions back and forth between LE ByteArrays and UIntX.
 def _root_.UInt8.toLEByteArray (n : UInt8) : ByteArray := ByteArray.mk #[n]
+def _root_.UInt8.toBEByteArray (n : UInt8) : ByteArray := ByteArray.mk #[n]
 
 def _root_.UInt16.toLEByteArray (n : UInt16) : ByteArray :=
   let b0 := (n      ).toUInt8
   let b1 := (n >>> 8).toUInt8
   ByteArray.mk #[b0, b1]
 
-def _root_.UInt16.toLEByteArray' (n : UInt16) : ByteArray :=
+def _root_.UInt16.toBEByteArray (n : UInt16) : ByteArray :=
   let b0 := (n      ).toUInt8
   let b1 := (n >>> 8).toUInt8
-  ByteArray.mk #[b0, b1]
+  ByteArray.mk #[b1, b0]
 
 def _root_.UInt32.toLEByteArray (n : UInt32) : ByteArray :=
   let b0 := (n       ).toUInt8
@@ -29,6 +30,13 @@ def _root_.UInt32.toLEByteArray (n : UInt32) : ByteArray :=
   let b2 := (n >>> 16).toUInt8
   let b3 := (n >>> 24).toUInt8
   ByteArray.mk #[b0, b1, b2, b3]
+
+def _root_.UInt32.toBEByteArray (n : UInt32) : ByteArray :=
+  let b0 := (n       ).toUInt8
+  let b1 := (n >>>  8).toUInt8
+  let b2 := (n >>> 16).toUInt8
+  let b3 := (n >>> 24).toUInt8
+  ByteArray.mk #[b3, b2, b1, b0]
 
 def _root_.UInt64.toLEByteArray (n : UInt64) : ByteArray :=
   let b0 := (n       ).toUInt8
@@ -41,9 +49,24 @@ def _root_.UInt64.toLEByteArray (n : UInt64) : ByteArray :=
   let b7 := (n >>> 56).toUInt8
   ByteArray.mk #[b0, b1, b2, b3, b4, b5, b6, b7]
 
+def _root_.UInt64.toBEByteArray (n : UInt64) : ByteArray :=
+  let b0 := (n       ).toUInt8
+  let b1 := (n >>>  8).toUInt8
+  let b2 := (n >>> 16).toUInt8
+  let b3 := (n >>> 24).toUInt8
+  let b4 := (n >>> 32).toUInt8
+  let b5 := (n >>> 40).toUInt8
+  let b6 := (n >>> 48).toUInt8
+  let b7 := (n >>> 56).toUInt8
+  ByteArray.mk #[b7, b6, b5, b4, b3, b2, b1, b0]
+
 def _root_.Int8.toLEByteArray (n : Int8) : ByteArray := n.toUInt8.toLEByteArray
 def _root_.Int16.toLEByteArray (n : Int16) : ByteArray := n.toUInt16.toLEByteArray
 def _root_.Int32.toLEByteArray (n : Int32) : ByteArray := n.toUInt32.toLEByteArray
 def _root_.Int64.toLEByteArray (n : Int64) : ByteArray := n.toUInt64.toLEByteArray
+def _root_.Int8.toBEByteArray (n : Int8) : ByteArray := n.toUInt8.toBEByteArray
+def _root_.Int16.toBEByteArray (n : Int16) : ByteArray := n.toUInt16.toBEByteArray
+def _root_.Int32.toBEByteArray (n : Int32) : ByteArray := n.toUInt32.toBEByteArray
+def _root_.Int64.toBEByteArray (n : Int64) : ByteArray := n.toUInt64.toBEByteArray
 
 end TensorLib
